Add missing [Axiom]s/[Lemma]s for our existing [model] files

theories/lang/cpp/model/simple_pred.v
@@ -1107,6 +1107,87 @@ Module SimpleCPP.
 
     Axiom exposed_aid_null_alloc_id : |-- exposed_aid null_alloc_id.
 
+    Lemma type_ptr_obj_repr_byte :
+      forall (σ : genv) (ty : type) (p : ptr) (i sz : N),
+        size_of σ ty = Some sz -> (* 1) [ty] has some byte-size [sz] *)
+        (i < sz)%N ->             (* 2) by (1), [sz] is nonzero and [i] is a
+                                        byte-offset into the object rooted at [p ,, o]
+
+                                     NOTE: [forall ty, size_of (Tarray ty 0) = Some 0],
+                                     but zero-length arrays are not permitted by the Standard
+                                     (cf. <https://eel.is/c++draft/dcl.array#def:array,bound>).
+                                     NOTE: if support for flexible array members is ever added,
+                                     it will need to be carefully coordinated with these sorts
+                                     of transport lemmas.
+                                   *)
+        (* 4) The existence of the "object representation" of an object of type [ty] -
+           |  in conjunction with the premises - justifies "lowering" any
+           |  [type_ptr ty p] fact to a collection of [type_ptr Tu8 (p ,, .[Tu8 ! i])]
+           |  facts - where [i] is a byte-offset within the [ty] ([0 <= i < sizeof(ty)]).
+           v *)
+        type_ptr ty p |-- type_ptr Tu8 (p ,, (o_sub σ Tu8 i)).
+    Proof. Admitted.
+
+    Lemma type_ptr_obj_repr :
+      forall (σ : genv) (ty : type) (p : ptr) (sz : N),
+        size_of σ ty = Some sz ->
+        type_ptr ty p |-- [∗list] i ∈ seqN 0 sz, type_ptr Tu8 (p ,, o_sub σ Tu8 (Z.of_N i)).
+    Proof.
+      intros * Hsz; iIntros "#tptr".
+      iApply big_sepL_intro; iIntros "!>" (k n) "%Hn'".
+      assert (lookup (K:=N) (N.of_nat k) (seqN 0%N sz) = Some n)
+        as Hn
+        by (unfold lookupN, list_lookupN; rewrite Nat2N.id //);
+        clear Hn'.
+      apply lookupN_seqN in Hn as [? ?].
+      iDestruct (type_ptr_obj_repr_byte σ ty p n sz Hsz ltac:(lia) with "tptr") as "$".
+    Qed.
+
+    (* [offset_congP] hoists [offset_cong] to [mpred] *)
+    Definition offset_congP (σ : genv) (o1 o2 : offset) : mpred :=
+      [| offset_cong σ o1 o2 |].
+
+    (* [ptr_congP σ p1 p2] is an [mpred] which quotients [ptr_cong σ p1 p2]
+       by requiring that [type_ptr Tu8] holds for both [p1] /and/ [p2]. This property
+       is intended to be sound and sufficient for transporting certain physical
+       resources between [p1] and [p2] - and we hypothesize that it is also
+       necessary.
+     *)
+    Definition ptr_congP (σ : genv) (p1 p2 : ptr) : mpred :=
+      [| ptr_cong σ p1 p2 |] ** type_ptr Tu8 p1 ** type_ptr Tu8 p2.
+
+    (* All [tptsto] facts can be transported over [ptr_congP] [ptr]s.
+
+       The standard justifies this as follows:
+       1) (cf. [tptsto] comment) [tptsto ty q p v] ensures that [p] points to a memory
+          location with C++ type [ty] and which has some value [v].
+       2) (cf. [Section type_ptr_object_representation]) [type_ptr Tu8] holds for all of the
+          bytes (i.e. the "object reprsentation") constituting well-typed C++ objects.
+       3) NOTE (JH): the following isn't quite true yet, but we'll want this when we flesh
+          out [rawR]/[RAW_BYTES]:
+          a) all values [v] can be converted into (potentially many) [raw_byte]s -
+             which capture its "object representation"
+          b) all [tptsto ty] facts can be shattered into (potentially many)
+             [tptsto Tu8 _ _ (Vraw _)] facts corresponding to its "object representation"
+       4) [tptsto Tu8 _ _ (Vraw _)] can be transported over [ptr_congP] [ptr]s:
+          a) [tptso Tu8 _ _ (Vraw _)] facts deal with the "object representation" directly
+             and thus permit erasing the structure of pointers in favor of reasoning about
+             relative byte offsets from a shared [ptr]-prefix.
+          b) the [ptr]s are [ptr_congP] so we know that:
+             i) they share a common base pointer [p_base]
+             ii) the byte-offset values of the C++ offsets which reconstitute the src/dst from
+                 [p_base] are equal
+             iii) NOTE: (cf. [valid_ptr_nonnull_nonzero]/[type_ptr_valid_ptr]/[type_ptr_nonnull] below)
+                  [p_base] has some [vaddr], but we don't currently rely on this fact.
+     *)
+    (* TODO: improve our axiomatic support for raw values - including "shattering"
+       non-raw values into their constituent raw pieces - to enable deriving
+       [tptsto_ptr_congP_transport] from [tptsto_raw_ptr_congP_transport].
+     *)
+    Lemma tptsto_ptr_congP_transport : forall {σ} ty q p1 p2 v,
+      ptr_congP σ p1 p2 |-- @tptsto σ ty q p1 v -* @tptsto σ ty q p2 v.
+    Proof. Admitted.
+
   End with_cpp.
 
 End SimpleCPP.
