theories/lang/cpp/model/inductive_pointers.v
@@ -588,6 +588,50 @@ Module PTRS_IMPL <: PTRS_INTF.
     all: done.
   Admitted.
 
+  Lemma ptr_common_prefix :
+    forall {p1 p2 : ptr} {o1 o2 : offset},
+      p1 ,, o1 = p2 ,, o2 ->
+      ∃ p oa ob,
+        p1 = p ,, oa /\ p2 = p ,, ob.
+  Proof.
+    intros p1 p2 o1 o2 Hps.
+    induction p1; rewrite _dot.unlock/DOT_dot/= in Hps; UNFOLD_dot.
+    - exists p2, o2, o_id; intuition; destruct p2=> //.
+    - admit. (* NOTE (JH): this lemma doesn't seem to hold for [fun_ptr_] *)
+    - destruct p2; destruct o2 as [[] ?]; simpl in *.
+      admit.
+  Admitted.
+
+  (* [eval_offset] respects the monoidal structure of [offset]s *)
+  Lemma eval_offset_dot : ∀ σ (o1 o2 : offset),
+    eval_offset σ (o1 ,, o2) =
+    add_opt (eval_offset σ o1) (eval_offset σ o2).
+  Proof. Admitted.
+
+  (* [ptr_vaddr] respects the right_monoid action of [__offset_ptr] *)
+  Lemma ptr_vaddr_dot : ∀ {σ} p (o : offset),
+    Z.of_N <$> ptr_vaddr (p ,, o) =
+    add_opt (Z.of_N <$> ptr_vaddr p) (eval_offset σ o).
+  Proof. Admitted.
+
+  (* not used. *)
+  Corollary ptr_vaddr_dot_derived {σ p o1 o2 va} :
+    same_property ptr_vaddr (p ,, o1) (p ,, o2) ->
+    ptr_vaddr p = Some va ->
+    same_property (eval_offset σ) o1 o2.
+  Proof.
+    rewrite !same_property_iff =>
+      -[va' []]
+       /(f_equal (fmap (M := option) Z.of_N)) +
+       /(f_equal (fmap (M := option) Z.of_N)) +
+       /= Hsome.
+    rewrite !ptr_vaddr_dot {}Hsome /=.
+    case: (eval_offset _ o1) (eval_offset _ o2) => [za|] [zb|] //.
+    cbn; intros Hza Hzb.
+    rewrite -{}Hzb in Hza; inversion Hza; clear Hza.
+    naive_solver eauto with f_equal lia.
+  Qed.
+
   Include PTRS_DERIVED_MIXIN.
   Include PTRS_MIXIN.
 End PTRS_IMPL.
